Update check_input_time

pancake/time_to_panScript.sml
@@ -1,6 +1,7 @@
 (*
   Compilation from timeLang to panLang
 *)
+
 open preamble pan_commonTheory mlintTheory
      timeLangTheory panLangTheory
 
@@ -18,7 +19,6 @@ End
 Definition ffiBufferAddr_def:
   ffiBufferAddr = 4000w:'a word
 End
-
 
 
 Definition ffiBufferSize_def:
@@ -197,8 +197,8 @@ Definition check_input_time_def:
   check_input_time =
     nested_seq [
         ExtCall «get_ffi» «ptr1» «len1» «ptr2» «len2» ;
-        Assign  «isInput» (Load One (Var «ptr2»)) ;
-        Assign  «sysTime» (Load One
+        Assign  «sysTime» (Load One (Var «ptr2»)) ;
+        Assign  «isInput» (Load One
                            (Op Add [Var «ptr2»;
                                     Const bytes_in_word]))
       ]
